Instantiator.v
@@ -1,8 +1,10 @@
 Require Import ObcToClight.Interface.
 Require Import Ident.
 Require Import Operators.
+Require Import Clocks.
 
 Module OpAux := OperatorsAux Op.
+Module Clks := ClocksFun Ids. 
 
 Require Import Coq.ZArith.BinInt.
 
@@ -12,11 +14,11 @@ Require Import NLustreToObc.Translation.
 Require Import NLustreToObc.Correctness.
 Require Import NLustreToObc.Fusible.
 
-Module NL := NLustreFun Ids Op OpAux.
+Module NL := NLustreFun Ids Op OpAux Clks.
 Module Obc := ObcFun Ids Op OpAux.
-Module Mem := MemoriesFun Ids Op NL.Syn.
-Module Trans := TranslationFun Ids Op OpAux NL.Syn Obc.Syn Mem.
-Module Typ := NLustreToObc.NLObcTyping.NLObcTypingFun Ids Op OpAux NL Obc Mem Trans.
-Module Corr := NLustreToObc.Correctness.CorrectnessFun Ids Op OpAux NL Obc Mem Trans Typ.
-Module Fusible := NLustreToObc.Fusible.FusibleFun Ids Op OpAux NL Obc Trans.
+Module Mem := MemoriesFun Ids Op Clks NL.Syn.
+Module Trans := TranslationFun Ids Op OpAux Clks NL.Syn Obc.Syn Mem.
+Module Typ := NLustreToObc.NLObcTyping.NLObcTypingFun Ids Op OpAux Clks NL Obc Mem Trans.
+Module Corr := NLustreToObc.Correctness.CorrectnessFun Ids Op OpAux Clks NL Obc Mem Trans Typ.
+Module Fusible := NLustreToObc.Fusible.FusibleFun Ids Op OpAux Clks NL Obc Trans.
 
