NLustre.v
@@ -1,4 +1,5 @@
 Require Import Operators.
+Require Import Clocks.
 Require Export NLustre.Stream.
 Require Export NLustre.NLSyntax.
 Require Export NLustre.IsFree.
@@ -18,59 +19,60 @@ Require Import NLustre.IsVariable.Decide.
 Require Import NLustre.IsDefined.Decide.
 Require Import NLustre.WellFormed.Decide.
 Require Import NLustre.IsFree.Decide.
-Require Export NLustre.Clocking.Parents.
 Require Export NLustre.Clocking.Properties.
 
 Module Type NLUSTRE
-       (Ids : IDS)
-       (Op  : OPERATORS)
-       (OpAux: OPERATORS_AUX Op).
-  Declare Module Export Syn: NLSYNTAX Ids Op.
+       (Ids   : IDS)
+       (Op    : OPERATORS)
+       (OpAux : OPERATORS_AUX Op)
+       (Clks  : CLOCKS Ids).
+  Declare Module Export Syn: NLSYNTAX Ids Op Clks.
   Declare Module Export Str: STREAM Op.
-  Declare Module Export Ord: ORDERED Ids Op Syn.
-  Declare Module Export IsF: ISFREE Ids Op Syn.
-  Declare Module Export IsFDec: IsFree.Decide.DECIDE Ids Op Syn IsF.
-  Declare Module Export Sem: NLSEMANTICS Ids Op OpAux Syn Str Ord.
-  Declare Module Export Typ: NLTYPING Ids Op Syn.
-  Declare Module Export Mem: MEMORIES Ids Op Syn.
-  Declare Module Export IsD: ISDEFINED Ids Op Syn Mem.
-  Declare Module Export IsV: ISVARIABLE Ids Op Syn Mem IsD.
-  Declare Module Export NoD: NODUP Ids Op Syn Mem IsD IsV.
-  Declare Module Export WeF: WELLFORMED Ids Op Syn IsF Ord Mem IsD IsV NoD.
-  Declare Module Export MemSem: MEMSEMANTICS Ids Op OpAux Syn Str Ord Mem IsF IsD Sem IsV NoD WeF.     
-  Declare Module Export IsVDec: IsVariable.Decide.DECIDE Ids Op Syn Mem IsD IsV.
-  Declare Module Export IsDDec: IsDefined.Decide.DECIDE Ids Op Syn Mem IsD.
-  Declare Module Export IsWFDec: WellFormed.Decide.DECIDE Ids Op Syn IsF IsFDec
+  Declare Module Export Ord: ORDERED Ids Op Clks Syn.
+  Declare Module Export IsF: ISFREE Ids Op Clks Syn.
+  Declare Module Export IsFDec: IsFree.Decide.DECIDE Ids Op Clks Syn IsF.
+  Declare Module Export Sem: NLSEMANTICS Ids Op OpAux Clks Syn Str Ord.
+  Declare Module Export Typ: NLTYPING Ids Op Clks Syn.
+  Declare Module Export Mem: MEMORIES Ids Op Clks Syn.
+  Declare Module Export IsD: ISDEFINED Ids Op Clks Syn Mem.
+  Declare Module Export IsV: ISVARIABLE Ids Op Clks Syn Mem IsD.
+  Declare Module Export NoD: NODUP Ids Op Clks Syn Mem IsD IsV.
+  Declare Module Export WeF: WELLFORMED Ids Op Clks Syn IsF Ord Mem IsD IsV NoD.
+  Declare Module Export MemSem: MEMSEMANTICS Ids Op OpAux Clks Syn Str Ord Mem
+                                    IsF IsD Sem IsV NoD WeF.     
+  Declare Module Export IsVDec: IsVariable.Decide.DECIDE Ids Op Clks Syn Mem IsD IsV.
+  Declare Module Export IsDDec: IsDefined.Decide.DECIDE Ids Op Clks Syn Mem IsD.
+  Declare Module Export IsWFDec: WellFormed.Decide.DECIDE Ids Op Clks Syn IsF IsFDec
                                      Ord Mem IsD IsV IsDDec IsVDec NoD WeF.
-  Declare Module Export Clo: CLOCKING Ids Op Syn.
-  Declare Module Export Par: PARENTS Ids Op Syn Clo.
-  Declare Module Export Pro: PROPERTIES Ids Op Syn IsF Clo Mem IsD Par.
+  Declare Module Export Clo: CLOCKING Ids Op Clks Syn.
+  Declare Module Export Pro: PROPERTIES Ids Op Clks Syn IsF Clo Mem IsD.
 End NLUSTRE.
 
 Module NLustreFun
-       (Import Ids   : IDS)
-       (Import Op    : OPERATORS)
-       (Import OpAux : OPERATORS_AUX Op)
-       <: NLUSTRE Ids Op OpAux.
-  Module Export Syn := NLSyntaxFun Ids Op.
-  Module Export Str := StreamFun Op.
-  Module Export Ord := OrderedFun Ids Op Syn.
-  Module Export IsF := IsFreeFun Ids Op Syn.
-  Module Export IsFDec := IsFree.Decide.DecideFun Ids Op Syn IsF.
-  Module Export Sem := NLSemanticsFun Ids Op OpAux Syn Str Ord.
-  Module Export Typ := NLTypingFun Ids Op Syn.
-  Module Export Mem := MemoriesFun Ids Op Syn.
-  Module Export IsD := IsDefinedFun Ids Op Syn Mem.
-  Module Export IsV := IsVariableFun Ids Op Syn Mem IsD.
-  Module Export NoD := NoDupFun Ids Op Syn Mem IsD IsV.
-  Module Export WeF := WellFormedFun Ids Op Syn IsF Ord Mem IsD IsV NoD.
-  Module Export MemSem := MemSemanticsFun Ids Op OpAux Syn Str Ord Mem IsF IsD Sem IsV NoD WeF.     
-  Module Export IsVDec := IsVariable.Decide.DecideFun Ids Op Syn Mem IsD IsV.
-  Module Export IsDDec := IsDefined.Decide.DecideFun Ids Op Syn Mem IsD.
-  Module Export IsWFDec := WellFormed.Decide.DecideFun Ids Op Syn IsF IsFDec Ord
-                                             Mem IsD IsV IsDDec IsVDec NoD WeF.
-  Module Export Clo := ClockingFun Ids Op Syn.
-  Module Export Par := ParentsFun Ids Op Syn Clo.
-  Module Export Pro := PropertiesFun Ids Op Syn IsF Clo Mem IsD Par.
+       (Ids   : IDS)
+       (Op    : OPERATORS)
+       (OpAux : OPERATORS_AUX Op)
+       (Clks  : CLOCKS Ids)
+       <: NLUSTRE Ids Op OpAux Clks.
+  Module Export Syn := NLSyntaxFun    Ids Op Clks.
+  Module Export Str := StreamFun          Op.
+  Module Export Ord := OrderedFun     Ids Op Clks Syn.
+  Module Export IsF := IsFreeFun      Ids Op Clks Syn.
+  Module Export IsFDec := IsFree.Decide.DecideFun Ids Op Clks Syn IsF.
+  Module Export Sem := NLSemanticsFun Ids Op OpAux Clks Syn Str Ord.
+  Module Export Typ := NLTypingFun    Ids Op Clks Syn.
+  Module Export Mem := MemoriesFun    Ids Op Clks Syn.
+  Module Export IsD := IsDefinedFun   Ids Op Clks Syn Mem.
+  Module Export IsV := IsVariableFun  Ids Op Clks Syn Mem IsD.
+  Module Export NoD := NoDupFun       Ids Op Clks Syn Mem IsD IsV.
+  Module Export WeF := WellFormedFun  Ids Op Clks Syn IsF Ord Mem IsD IsV NoD.
+  Module Export MemSem := MemSemanticsFun Ids Op OpAux Clks Syn Str Ord Mem IsF
+                            IsD Sem IsV NoD WeF.     
+  Module Export IsVDec := IsVariable.Decide.DecideFun Ids Op Clks Syn Mem IsD IsV.
+  Module Export IsDDec := IsDefined.Decide.DecideFun Ids Op Clks Syn Mem IsD.
+  Module Export IsWFDec := WellFormed.Decide.DecideFun Ids Op Clks Syn IsF
+                            IsFDec Ord Mem IsD IsV IsDDec IsVDec NoD WeF.
+  Module Export Clo := ClockingFun    Ids Op Clks Syn.
+  Module Export Pro := PropertiesFun  Ids Op Clks Syn IsF Clo Mem IsD.
 End NLustreFun.
 
