NLustre/Clocking/Properties.v
@@ -1,22 +1,22 @@
 Require Import Velus.Common.
 Require Import Velus.Operators.
+Require Import Velus.Clocks.
 Require Import NLustre.NLSyntax.
 Require Import NLustre.Clocking.
-Require Import NLustre.Clocking.Parents.
 
 Require Import NLustre.IsFree.
 Require Import NLustre.IsDefined.
 Require Import NLustre.Memories.
 
 Module Type PROPERTIES
-       (Ids : IDS)
-       (Op  : OPERATORS)
-       (Import Syn : NLSYNTAX Ids Op)
-       (Import IsF : ISFREE Ids Op Syn)
-       (Import Clo : CLOCKING Ids Op Syn)
-       (Mem        : MEMORIES Ids Op Syn)
-       (Import IsD : ISDEFINED Ids Op Syn Mem)
-       (Import Par : PARENTS Ids Op Syn Clo).
+       (Ids         : IDS)
+       (Op          : OPERATORS)
+       (Import Clks : CLOCKS Ids)
+       (Import Syn  : NLSYNTAX  Ids Op Clks)
+       (Import IsF  : ISFREE    Ids Op Clks Syn)
+       (Import Clo  : CLOCKING  Ids Op Clks Syn)
+       (Mem         : MEMORIES  Ids Op Clks Syn)
+       (Import IsD  : ISDEFINED Ids Op Clks Syn Mem).
 
   Lemma Is_free_in_clock_self_or_parent:
     forall x ck,
@@ -32,6 +32,25 @@ Module Type PROPERTIES
       destruct IH as [ck' [b' Hcp]].
       exists ck', b'; right.
       destruct Hcp as [Hcp|Hcp]; [rewrite Hcp| inversion Hcp]; now auto.
+  Qed.
+
+  Lemma wc_clock_parent:
+    forall C ck' ck,
+      wc_env C
+      -> clock_parent ck ck'
+      -> wc_clock C ck'
+      -> wc_clock C ck.
+  Proof.
+    Hint Constructors wc_clock.
+    induction ck' as [|ck' IH]; destruct ck as [|ck i' ty' b'];
+    try now (inversion 3 || auto).
+    intros Hwc Hp Hck.
+    inversion Hp as [j c [HR1 HR2 HR3]|ck'' j c Hp' [HR1 HR2 HR3]].
+    - rewrite <-HR1 in *; clear HR1 HR2 HR3.
+      now inversion_clear Hck.
+    - subst.
+      apply IH with (1:=Hwc) (2:=Hp').
+      now inversion Hck.
   Qed.
   
   Section Well_clocked.
@@ -130,14 +149,14 @@ Module Type PROPERTIES
 End PROPERTIES.
 
 Module PropertiesFun
-       (Ids : IDS)
-       (Op  : OPERATORS)
-       (Import Syn : NLSYNTAX Ids Op)
-       (Import IsF : ISFREE Ids Op Syn)
-       (Import Clo : CLOCKING Ids Op Syn)
-       (Mem        : MEMORIES Ids Op Syn)
-       (Import IsD : ISDEFINED Ids Op Syn Mem)
-       (Import Par : PARENTS Ids Op Syn Clo)
-       <: PROPERTIES Ids Op Syn IsF Clo Mem IsD Par.
-  Include PROPERTIES Ids Op Syn IsF Clo Mem IsD Par.
+       (Ids  : IDS)
+       (Op   : OPERATORS)
+       (Clks : CLOCKS    Ids)
+       (Syn  : NLSYNTAX  Ids Op Clks)
+       (IsF  : ISFREE    Ids Op Clks Syn)
+       (Clo  : CLOCKING  Ids Op Clks Syn)
+       (Mem  : MEMORIES  Ids Op Clks Syn)
+       (IsD  : ISDEFINED Ids Op Clks Syn Mem)
+       <: PROPERTIES Ids Op Clks Syn IsF Clo Mem IsD.
+  Include PROPERTIES Ids Op Clks Syn IsF Clo Mem IsD.
 End PropertiesFun.
