NLustre/IsDefined/Decide.v
@@ -6,6 +6,7 @@ Open Scope list_scope.
 
 Require Import Velus.Common.
 Require Import Velus.Operators.
+Require Import Velus.Clocks.
 Require Import Velus.NLustre.NLSyntax.
 Require Import Velus.NLustre.IsDefined.
 Require Import Velus.NLustre.Memories.
@@ -20,11 +21,12 @@ is equivalent to its specification.
  *)
 
 Module Type DECIDE
-       (Ids : IDS)
-       (Op  : OPERATORS)
-       (Import Syn : NLSYNTAX Ids Op)
-       (Import Mem : MEMORIES Ids Op Syn)
-       (Import IsD : ISDEFINED Ids Op Syn Mem).
+       (Ids         : IDS)
+       (Op          : OPERATORS)
+       (Import Clks : CLOCKS    Ids)
+       (Import Syn  : NLSYNTAX  Ids Op Clks)
+       (Import Mem  : MEMORIES  Ids Op Clks Syn)
+       (Import IsD  : ISDEFINED Ids Op Clks Syn Mem).
 
   (** ** Decision procedures: *)
 
@@ -304,13 +306,12 @@ Module Type DECIDE
 End DECIDE.
 
 Module DecideFun
-       (Ids : IDS)
-       (Op  : OPERATORS)
-       (Import Syn : NLSYNTAX Ids Op)
-       (Import Mem : MEMORIES Ids Op Syn)
-       (Import IsD : ISDEFINED Ids Op Syn Mem)
-       <: DECIDE Ids Op Syn Mem IsD.
-
-  Include DECIDE Ids Op Syn Mem IsD.
-
+       (Ids  : IDS)
+       (Op   : OPERATORS)
+       (Clks : CLOCKS    Ids)
+       (Syn  : NLSYNTAX  Ids Op Clks)
+       (Mem  : MEMORIES  Ids Op Clks Syn)
+       (IsD  : ISDEFINED Ids Op Clks Syn Mem)
+       <: DECIDE Ids Op Clks Syn Mem IsD.
+  Include DECIDE Ids Op Clks Syn Mem IsD.
 End DecideFun.
