NLustreToObc/Correctness.v
@@ -4,6 +4,7 @@ Open Scope list_scope.
 
 Require Import Velus.Common.
 Require Import Velus.Operators.
+Require Import Velus.Clocks.
 Open Scope positive.
 
 Require Import Velus.RMemory.
@@ -18,15 +19,16 @@ Module Type CORRECTNESS
        (Import Ids   : IDS)
        (Import Op    : OPERATORS)
        (Import OpAux : OPERATORS_AUX Op)
-       (Import DF    : NLUSTRE Ids Op OpAux)
-       (Import Obc   : OBC Ids Op OpAux)
-       (Import Mem   : MEMORIES Ids Op DF.Syn)
+       (Import Clks  : CLOCKS    Ids)
+       (Import DF    : NLUSTRE   Ids Op OpAux Clks)
+       (Import Obc   : OBC       Ids Op OpAux)
+       (Import Mem   : MEMORIES  Ids Op       Clks DF.Syn)
 
-       (Import Trans : TRANSLATION Ids Op OpAux DF.Syn Obc.Syn Mem)
-       (Import NLObcTyping: NLOBCTYPING Ids Op OpAux DF Obc Mem Trans).
+       (Import Trans : TRANSLATION Ids Op OpAux Clks DF.Syn Obc.Syn Mem)
+       (Import NLObcTyping: NLOBCTYPING Ids Op OpAux Clks DF Obc Mem Trans).
 
-  Module Import IsP := IsPresentFun Ids Op OpAux DF.Syn Obc.Syn Obc.Sem Mem Trans.
-  Module Import MemCor := MemoryCorresFun Ids Op OpAux DF Obc.
+  Module Import IsP := IsPresentFun Ids Op OpAux Clks DF.Syn Obc.Syn Obc.Sem Mem Trans.
+  Module Import MemCor := MemoryCorresFun Ids Op OpAux Clks DF Obc.
   
   (** ** Technical lemmas *)
 
@@ -2235,17 +2237,15 @@ for all [Is_free_exp x e]. *)
 End CORRECTNESS.
 
 Module CorrectnessFun
-       (Import Ids   : IDS)
-       (Import Op    : OPERATORS)
-       (Import OpAux : OPERATORS_AUX Op)
-       (Import DF    : NLUSTRE Ids Op OpAux)
-       (Import Obc   : OBC Ids Op OpAux)
-       (Import Mem   : MEMORIES Ids Op DF.Syn)
-       (Import Trans : TRANSLATION Ids Op OpAux DF.Syn Obc.Syn Mem)
-       (Import NLObcTyping: NLOBCTYPING Ids Op OpAux DF Obc Mem Trans)
-
-       <: CORRECTNESS Ids Op OpAux DF Obc Mem Trans NLObcTyping.
-
-  Include CORRECTNESS Ids Op OpAux DF Obc Mem Trans NLObcTyping.
-
+       (Ids         : IDS)
+       (Op          : OPERATORS)
+       (OpAux       : OPERATORS_AUX   Op)
+       (Clks        : CLOCKS      Ids)
+       (DF          : NLUSTRE     Ids Op OpAux Clks)
+       (Obc         : OBC         Ids Op OpAux)
+       (Mem         : MEMORIES    Ids Op       Clks DF.Syn)
+       (Trans       : TRANSLATION Ids Op OpAux Clks DF.Syn Obc.Syn Mem)
+       (NLObcTyping : NLOBCTYPING Ids Op OpAux Clks DF Obc Mem Trans)
+       <: CORRECTNESS Ids Op OpAux Clks DF Obc Mem Trans NLObcTyping.
+  Include CORRECTNESS Ids Op OpAux Clks DF Obc Mem Trans NLObcTyping.
 End CorrectnessFun.
